refactoring

Coq/src/EventStructure.v
@@ -116,6 +116,13 @@ Definition cont_cf_dom S c :=
   | CEvent e => dom_rel (cf S ⨾ ⦗ eq e ⦘) ∪₁ codom_rel (⦗ eq e ⦘ ⨾ sb S)
   end.
 
+Definition cont_adjacent S k k' e e' := 
+  ⟪ kREP' : k' = CEvent (opt_ext e e') ⟫ /\ 
+  ⟪ kEQTID : ES.cont_thread S k = ES.cont_thread S k' ⟫ /\
+  ⟪ nINITe : ES.acts_ninit_set S e ⟫ /\
+  ⟪ RMWe : eq e × eq_opt e' ⊆ ES.rmw S ⟫ /\
+  ⟪ kSBDOM : ES.cont_sb_dom S k ≡₁ dom_rel (ES.sb S ⨾ ⦗eq e⦘) ⟫.
+
 (* An initial event structure. *)
 Definition init loc_list conts :=
   let loc_labs := map init_write loc_list in
@@ -299,6 +306,9 @@ Implicit Type WF : Wf.
 (** ** acts_set properties *)
 (******************************************************************************)
 
+Lemma E_alt : E ≡₁ fun x => List.In x (first_nat_list S.(next_act)).
+Proof. red; split; red; apply first_nat_list_In_alt. Qed.
+
 Lemma acts_set_split : E ≡₁ Einit ∪₁ Eninit.
 Proof.
   unfold ES.acts_init_set, ES.acts_ninit_set.
@@ -369,6 +379,38 @@ Proof.
   apply inclusion_union_l; basic_solver. 
 Qed.
 
+Lemma sb_clos_imm_split WF : sb ≡ (immediate sb)⁺.
+Proof.
+  eapply ct_imm1.
+  { apply WF.(sb_irr). }
+  { apply WF.(sb_trans). }
+  rewrite (dom_l WF.(sbE)).
+  rewrite dom_seq, dom_eqv, E_alt.
+  reflexivity.
+Qed.
+
+Lemma sb_imm_split_r WF : sb ≡ sb^? ⨾ immediate sb.
+Proof.
+  split.
+  2: { generalize WF.(sb_trans). basic_solver. }
+  rewrite sb_clos_imm_split at 1; auto.
+  rewrite ct_end.
+  apply seq_mori; [|done].
+  rewrite immediate_in.
+  apply rt_of_trans. by apply sb_trans.
+Qed.
+
+Lemma sb_imm_split_l WF : sb ≡ immediate sb ⨾ sb^?.
+Proof.
+  split.
+  2: { generalize WF.(sb_trans). basic_solver. }
+  rewrite sb_clos_imm_split at 1; auto.
+  rewrite ct_begin.
+  apply seq_mori; [done|].
+  rewrite immediate_in.
+  apply rt_of_trans. by apply sb_trans.
+Qed.
+
 Lemma Tid_sb_prcl WF t : 
   dom_rel (sb ⨾ ⦗Tid_ t⦘) ⊆₁ Einit ∪₁ Tid_ t.
 Proof. 
@@ -425,6 +467,36 @@ Proof.
   unfolder; split; auto. 
   apply sbE in SB; auto. 
   generalize SB. basic_solver.
+Qed.
+
+Lemma immediate_tsb_functional WF x y z 
+      (nINITy  : Eninit y)
+      (IMMtSB  : immediate (sb)⁻¹ x y)
+      (IMMtSB' : immediate (sb)⁻¹ x z) : 
+  y = z.
+Proof. 
+  destruct IMMtSB  as [SB  nSB ].
+  destruct IMMtSB' as [SB' nSB'].
+  unfold transp in *.
+  assert (Eninit z) as nINITz.
+  { red. split.
+    { apply sbE in SB'; auto.
+      generalize SB'. basic_solver. }
+    intros INITz.
+    eapply (nSB' y); auto.
+    apply sb_init; auto.
+    basic_solver. }
+  edestruct sb_prcl 
+    as [EQ | HH]; eauto.
+  { split; eauto.
+    eapply sb_tid; auto.
+    basic_solver. }
+  { split; eauto.
+    eapply sb_tid; auto.
+    basic_solver. }
+  destruct HH as [[HH _] | [HH _]].
+  { exfalso. eapply nSB; eauto. }
+  exfalso. eapply (nSB' y); auto.
 Qed.
 
 (******************************************************************************)
@@ -1335,6 +1407,108 @@ Proof.
 Qed.
 
 (******************************************************************************)
+(** ** cont_adjacent properites *)
+(******************************************************************************)
+
+Lemma cont_adjacent_rmw WF k k' e e' 
+      (ADJ : cont_adjacent S k k' e (Some e')) :
+  rmw e e'.
+Proof. 
+  unfold cont_adjacent in ADJ; desc. 
+  apply RMWe. basic_solver.
+Qed.
+
+Lemma cont_adjacent_ninit_e WF k k' e e' 
+      (ADJ : cont_adjacent S k k' e e') :
+  Eninit e.
+Proof. by unfold cont_adjacent in ADJ; desc. Qed.
+
+Lemma cont_adjacent_ninit_e' WF k k' e e' 
+      (ADJ : cont_adjacent S k k' e (Some e')) :
+  Eninit e'.
+Proof. 
+  pose proof (cont_adjacent_rmw WF ADJ) as RMW.
+  apply rmwEninit in RMW; auto.
+  generalize RMW. basic_solver. 
+Qed.
+
+Lemma cont_adjacent_tid_e WF k k' e e' 
+      (ADJ : cont_adjacent S k k' e e') :
+  tid e = ES.cont_thread S k.
+Proof. 
+  unfold cont_adjacent in ADJ; desc.
+  rewrite kEQTID. subst k'.
+  unfold ES.cont_thread, opt_ext in *.
+  destruct e' as [e'|]; auto.
+  apply rmwt; auto.
+  apply RMWe. basic_solver. 
+Qed.
+
+Lemma cont_adjacent_tid_e' WF k k' e e' 
+      (ADJ : cont_adjacent S k k' e (Some e')) :
+  tid e' = ES.cont_thread S k.
+Proof. 
+  unfold cont_adjacent in ADJ; desc.
+  rewrite kEQTID. subst k'.
+  unfold ES.cont_thread, opt_ext in *; auto.
+Qed.
+
+Lemma cont_adjacent_sb_dom WF k k' e e'
+      (ADJ : cont_adjacent S k k' e e') :
+  ES.cont_sb_dom S k' ≡₁ ES.cont_sb_dom S k ∪₁ eq e ∪₁ eq_opt e'.
+Proof. 
+  red in ADJ. desc. subst k'.
+  unfold ES.cont_sb_dom at 1.
+  unfold opt_ext, eq_opt in *.
+  destruct e' as [e'|].
+
+  { assert (rmw e e') as RMW.
+    { generalize RMWe. basic_solver. }
+    rewrite crE. relsf.
+    rewrite set_unionC.
+    apply set_union_Propere; auto.
+    arewrite (dom_rel (sb ⨾ ⦗eq e'⦘) ≡₁ 
+                      dom_rel (sb^? ⨾ ⦗eq e⦘)).
+    { split.
+      { rewrite sb_imm_split_r at 1; auto. 
+        rewrite !seqA, !seq_eqv_r.
+        intros x [y [z [SB [IMMSB EQy]]]].
+        subst y. exists z. 
+        splits; auto.
+        eapply immediate_tsb_functional; eauto.
+        { apply immediate_transp with (r := sb). red.
+          eapply rmwi; eauto. }
+        apply immediate_transp with (r := sb). by red. }
+      rewrite crE. relsf. 
+      rewrite !seq_eqv_r. splits.
+      { unfolder. ins. desf.
+        eexists; splits; eauto.
+        apply rmw_in_sb; auto. }
+      unfolder. ins. desf.
+      exists e'; splits; eauto.
+      eapply sb_trans; eauto.
+      apply rmw_in_sb; auto. }
+    rewrite crE. relsf.
+    rewrite set_unionC.
+    apply set_union_Propere; auto.
+      by rewrite kSBDOM. }
+
+  rewrite crE. relsf.
+  rewrite set_unionC.
+  apply set_union_Propere; auto.
+    by rewrite kSBDOM.
+Qed.
+
+Lemma cont_adjacent_sb_dom_mon WF k k' e e'
+      (ADJ : cont_adjacent S k k' e e') :
+  ES.cont_sb_dom S k ⊆₁ ES.cont_sb_dom S k'.
+Proof. 
+  erewrite cont_adjacent_sb_dom 
+    with (k' := k'); eauto.
+  basic_solver.
+Qed.
+
+(******************************************************************************)
 (** ** seqn properites *)
 (******************************************************************************)
 
@@ -1411,9 +1585,6 @@ Proof.
   eapply seqn_sb_alt; eauto.
 Qed.
 
-Lemma E_alt : E ≡₁ fun x => List.In x (first_nat_list S.(next_act)).
-Proof. red; split; red; apply first_nat_list_In_alt. Qed.
-
 Lemma sb_well_founded WF : well_founded sb.
 Proof.
   apply fsupp_well_founded.
@@ -1432,38 +1603,6 @@ Proof.
   red. ins.
   eexists. intros. apply E_alt.
   apply WF.(sbE) in REL. by destruct_seq REL as [YY XX].
-Qed.
-
-Lemma sb_clos_imm_split WF : sb ≡ (immediate sb)⁺.
-Proof.
-  eapply ct_imm1.
-  { apply WF.(sb_irr). }
-  { apply WF.(sb_trans). }
-  rewrite (dom_l WF.(sbE)).
-  rewrite dom_seq, dom_eqv, E_alt.
-  reflexivity.
-Qed.
-
-Lemma sb_imm_split_r WF : sb ≡ sb^? ⨾ immediate sb.
-Proof.
-  split.
-  2: { generalize WF.(sb_trans). basic_solver. }
-  rewrite sb_clos_imm_split at 1; auto.
-  rewrite ct_end.
-  apply seq_mori; [|done].
-  rewrite immediate_in.
-  apply rt_of_trans. by apply sb_trans.
-Qed.
-
-Lemma sb_imm_split_l WF : sb ≡ immediate sb ⨾ sb^?.
-Proof.
-  split.
-  2: { generalize WF.(sb_trans). basic_solver. }
-  rewrite sb_clos_imm_split at 1; auto.
-  rewrite ct_begin.
-  apply seq_mori; [done|].
-  rewrite immediate_in.
-  apply rt_of_trans. by apply sb_trans.
 Qed.
 
 Lemma seqn_after_null_imm WF y (EE : Eninit y) :
