Coq/src/SimRelCertStepLemma.v
@@ -148,6 +148,142 @@ Section SimRelCertStepLemma.
 
   Notation "'certX' S" := (fun k => (X ∩₁ SNTid_ S (ktid S k)) ∪₁ (kE S k)) (at level 1, only parsing).
 
+    Definition forwarding S lbl lbl' k k' e e'
+             (st st' : thread_st (ktid S k)) :=
+    ⟪ LBL  : lbl  = Slab S e ⟫ /\
+    ⟪ LBL' : lbl' = option_map (Slab S) e' ⟫ /\
+    ⟪ Kk   : K S (k , existT _ _ st ) ⟫ /\
+    ⟪ Kk'  : K S (k', existT _ _ st') ⟫ /\
+    ⟪ ADJ  : ES.cont_adjacent S k k' e e'⟫ /\
+    ⟪ STEP : ilbl_step (ktid S k) (opt_to_list lbl' ++ [lbl]) st st' ⟫ /\  
+    ⟪ CertRF : e2a S □ Sjf S ⨾ ⦗eq e⦘ ⊆ cert_rf G sc TC' (ktid S k) ⟫.  
+
+  Lemma forwarding_seqn_e S lbl lbl' k k' e e'
+             (st st' st'': thread_st (ktid S k))
+             (SRCC : simrel_cert prog S G sc TC TC' X k st st'')
+             (FRWD : forwarding S lbl lbl' k k' e e' st st') :
+    ES.seqn S e = eindex st.
+  Proof. 
+    assert (ES.Wf S) as WF.
+    { apply SRCC. }
+    assert (simrel_cont (stable_prog_to_prog prog) S G TC X) 
+      as SRCONT.
+    { apply SRCC. }
+    unfold forwarding in FRWD. desc.
+    set (AA := ADJ).
+    unfold ES.cont_adjacent in AA. desc.
+    unfold ES.cont_sb_dom in kSBDOM.
+    destruct k eqn:Heq.
+    { erewrite continit; eauto.
+      unfold ES.seqn.
+      arewrite (dom_rel (Ssb S ∩ ES.same_tid S ⨾ ⦗eq e⦘) ≡₁ ∅).
+      2 : by erewrite countNatP_empty.
+      split; [|done].
+      rewrite seq_eqv_r.
+      intros x [y [[SB STID] EQy]].
+      red. subst y.
+      eapply ES.init_tid_K; eauto.
+      exists (existT _ _ st), k.
+      splits; [by subst k|]. 
+      subst k. erewrite <- ES.cont_adjacent_tid_e; eauto.
+      rewrite <- STID.
+      assert (SEinit S x) as INITx.
+      { apply kSBDOM. basic_solver 10. }
+      red in INITx. unfolder in INITx. desf. }
+    erewrite contseqn; eauto.
+    erewrite ES.seqn_immsb; eauto.
+    { red. 
+      erewrite ES.cont_adjacent_tid_e 
+        with (k := k) (e := e); eauto.
+      2 : eby subst k.
+      unfold ES.cont_thread. desf. }
+    red. splits.
+    { assert (dom_rel (Ssb S ⨾ ⦗eq e⦘) eid) as HH.
+      { apply kSBDOM. basic_solver 10. }
+      unfolder in HH. desf. } 
+    intros x SB SB'.
+    assert (dom_rel ((Ssb S)^? ⨾ ⦗eq eid⦘) x) as HH.
+    { apply kSBDOM. basic_solver 10. }
+    unfolder in HH. desf.
+    { eapply ES.sb_irr; eauto. }
+    eapply ES.sb_irr; eauto.
+    eapply ES.sb_trans; eauto.
+  Qed.
+
+  Lemma forwarding_seqn_e' S lbl lbl' k k' e e'
+        (st st' st'': thread_st (ktid S k))
+        (SRCC : simrel_cert prog S G sc TC TC' X k st st'')
+        (FRWD : forwarding S lbl lbl' k k' e (Some e') st st') :
+    ES.seqn S e' = 1 + eindex st.
+  Proof. 
+    assert (ES.Wf S) as WF.
+    { apply SRCC. }
+    assert (simrel_cont (stable_prog_to_prog prog) S G TC X) 
+      as SRCONT.
+    { apply SRCC. }
+    set (AA := FRWD).
+    unfold forwarding in AA. desc.
+    set (AA := ADJ).
+    unfold ES.cont_adjacent in AA. desc.
+    assert (immediate (ES.sb S) e e') as IMMSB.
+    { apply ES.rmwi; auto.
+      apply RMWe. basic_solver. }
+    erewrite ES.seqn_immsb 
+      with (x := e); eauto; try red; splits.
+    { erewrite forwarding_seqn_e; eauto. }
+    erewrite ES.cont_adjacent_tid_e; eauto. 
+    erewrite ES.cont_adjacent_tid_e'
+      with (k := k); eauto. 
+  Qed.
+
+  Lemma forwarding_e2a_e S lbl lbl' k k' e e'
+             (st st' st'': thread_st (ktid S k))
+             (SRCC : simrel_cert prog S G sc TC TC' X k st st'')
+             (FRWD : forwarding S lbl lbl' k k' e e' st st') :
+    e2a S e = ThreadEvent (ES.cont_thread S k) (eindex st).
+  Proof. 
+    assert (ES.Wf S) as WF.
+    { apply SRCC. }
+    assert (ES.cont_adjacent S k k' e e') as ADJ.
+    { apply FRWD. }
+    rewrite e2a_ninit; auto.
+    2 : eapply ES.cont_adjacent_ninit_e; eauto.
+    erewrite ES.cont_adjacent_tid_e; eauto.
+    erewrite forwarding_seqn_e; eauto.
+  Qed.
+
+  Lemma forwarding_e2a_e' S lbl lbl' k k' e e'
+        (st st' st'': thread_st (ktid S k))
+        (SRCC : simrel_cert prog S G sc TC TC' X k st st'')
+        (FRWD : forwarding S lbl lbl' k k' e (Some e') st st') :
+    e2a S e' = ThreadEvent (ES.cont_thread S k) (1 + eindex st).
+  Proof. 
+    assert (ES.Wf S) as WF.
+    { apply SRCC. }
+    assert (ES.cont_adjacent S k k' e (Some e')) as ADJ.
+    { apply FRWD. }
+    rewrite e2a_ninit; auto.
+    2 : eapply ES.cont_adjacent_ninit_e'; eauto.
+    erewrite ES.cont_adjacent_tid_e'; eauto.
+    erewrite forwarding_seqn_e'; eauto.
+  Qed.
+
+  Lemma simrel_cert_forwarding_ex_ktid_cov lbl lbl' k k' e e' S 
+        (st st' st'': (thread_st (ktid S k)))
+        (SRCC : simrel_cert prog S G sc TC TC' X k st st'') 
+        (FRWD : forwarding S lbl lbl' k k' e e' st st')         
+        (CST_REACHABLE : (lbl_step (ktid S k))＊ st' st'') :
+    X ∩₁ Stid_ S (ktid S k') ∩₁ e2a S ⋄₁ C ⊆₁ kE S k'. 
+  Proof. 
+    assert (ES.Wf S) as WF.
+    { apply SRCC. }
+    arewrite (ktid S k' = ktid S k).
+    { symmetry. apply FRWD. }
+    etransitivity; [apply SRCC|].
+    eapply ES.cont_adjacent_sb_dom_mon; eauto.
+    apply FRWD.
+  Qed.
+
   Lemma simrel_cert_step_ex_ktid_cov k k' e e' S S'
         (st st' st'': (thread_st (ktid S k)))
         (SRCC : simrel_cert prog S G sc TC TC' X k st st'') 
@@ -171,6 +307,41 @@ Section SimRelCertStepLemma.
     erewrite Execution.ex_inE 
       with (X := X); eauto.
     basic_solver. 
+  Qed.
+  
+  Lemma simrel_cert_forwarding_cov_in_ex lbl lbl' k k' e e' S 
+        (st st' st'': (thread_st (ktid S k)))
+        (SRCC : simrel_cert prog S G sc TC TC' X k st st'') 
+        (FRWD : forwarding S lbl lbl' k k' e e' st st')         
+        (CST_REACHABLE : (lbl_step (ktid S k))＊ st' st'') :
+    e2a S ⋄₁ C ∩₁ kE S k' ⊆₁ X.
+  Proof. 
+    assert (ES.Wf S) as WF.
+    { apply SRCC. }
+    assert (ES.cont_adjacent S k k' e e') as ADJ.
+    { apply FRWD. }
+    rewrite ES.cont_adjacent_sb_dom 
+      with (k' := k'); eauto.
+    rewrite set_unionA.
+    rewrite set_inter_union_r.
+    unionL.
+    { rewrite set_interC. 
+      rewrite set_interC. 
+      apply SRCC. }
+    rewrite set_inter_union_r. 
+    unfolder. unionL.
+    { intros x [Cx EQx]. subst x. exfalso. 
+      eapply e2a_ge_ncov; eauto.
+      { apply FRWD. }
+      { erewrite ES.cont_adjacent_tid_e; eauto. }
+      erewrite forwarding_seqn_e; eauto. }
+    intros x [Cx EQx].
+    destruct e' as [e'|]; [|done].
+    subst x. exfalso. 
+    eapply e2a_ge_ncov; eauto.
+    { eapply ES.cont_adjacent_ninit_e'; eauto. }
+    { erewrite ES.cont_adjacent_tid_e'; eauto. }
+    erewrite forwarding_seqn_e'; eauto. 
   Qed.
 
   Lemma simrel_cert_step_cov_in_ex k k' e e' S S'
@@ -210,6 +381,81 @@ Section SimRelCertStepLemma.
     omega.
   Qed.
 
+  Lemma simrel_cert_forwarding_kE_lab lbl lbl' k k' e e' S 
+        (st st' st'': (thread_st (ktid S k)))
+        (SRCC : simrel_cert prog S G sc TC TC' X k st st'') 
+        (FRWD : forwarding S lbl lbl' k k' e e' st st')         
+        (CST_REACHABLE : (lbl_step (ktid S k))＊ st' st'') :
+    eq_dom (kE S k' \₁ SEinit S) (Slab S) (Execution.lab (ProgToExecution.G st'') ∘ e2a S).
+  Proof. 
+    assert (ES.Wf S) as WF.
+    { apply SRCC. }
+    assert (simrel_cont (stable_prog_to_prog prog) S G TC X) 
+      as SRCONT.
+    { apply SRCC. } 
+    assert (ES.cont_adjacent S k k' e e') as ADJ.
+    { apply FRWD. }
+    set (AA := FRWD).
+    cdes AA.
+    assert (ktid S k = ktid S k') as kEQTID.
+    { by apply ADJ. }
+    assert (wf_thread_state (ktid S k) st) as WFst.
+    { eapply contwf; eauto. }
+    assert (wf_thread_state (ktid S k) st') as WFst'.
+    { rewrite kEQTID. eapply contwf; eauto. by rewrite <- kEQTID. }
+    assert (Gtid (e2a S e) = ES.cont_thread S k) as GTIDe.
+    { erewrite e2a_ninit; [|apply ADJ].
+      unfold Events.tid.
+      erewrite ES.cont_adjacent_tid_e; eauto. }
+    rewrite ES.cont_adjacent_sb_dom 
+      with (k' := k'); eauto.
+    rewrite set_unionA.
+    rewrite !set_minus_union_l.
+    rewrite !eq_dom_union. splits.
+    { apply SRCC. }
+    { intros x [EQx _]. subst x.
+      unfold compose.
+      erewrite steps_preserve_lab; eauto.
+      { rewrite <- LBL.
+        erewrite forwarding_e2a_e; eauto.
+        eapply ilbl_step_eindex_lbl; eauto. }
+      { by rewrite GTIDe. }
+      { apply lbl_steps_in_steps. 
+          by rewrite GTIDe. }
+      erewrite forwarding_e2a_e; eauto.
+      eapply acts_clos; eauto.
+      eapply ilbl_step_eindex_lt.
+      apply STEP. }
+    intros x [EQx _]. 
+    unfold eq_opt in EQx. 
+    destruct e' as [e'|]; [|done]. 
+    assert (Gtid (e2a S e') = ES.cont_thread S k) as GTIDe'.
+    { erewrite e2a_ninit.
+      2 : eapply ES.cont_adjacent_ninit_e'; eauto.
+      unfold Events.tid.
+      erewrite ES.cont_adjacent_tid_e'; eauto. }
+    subst x. unfold compose.
+    erewrite steps_preserve_lab; eauto.
+    { unfold option_map in LBL'.
+      destruct lbl' as [lbl'|]; 
+        inversion LBL' as [HLBL'].
+      rewrite <- HLBL'.
+      erewrite forwarding_e2a_e'; eauto.
+      eapply ilbl_step_eindex_lbl'; eauto. }
+    { by rewrite GTIDe'. }
+    { apply lbl_steps_in_steps. 
+        by rewrite GTIDe'. }
+    erewrite forwarding_e2a_e'; eauto.
+    eapply acts_clos; eauto.
+    erewrite ilbl_step_eindex_shift
+      with (st' := st'); eauto.
+    unfold option_map in LBL'.
+    destruct lbl' as [lbl'|].
+    2 : inversion LBL'.
+    unfold opt_to_list, app, length.
+    omega. 
+  Qed.
+
   Lemma simrel_cert_step_kE_lab k k' e e' S S'
         (st st' st'': (thread_st (ktid S k)))
         (SRCC : simrel_cert prog S G sc TC TC' X k st st'')
@@ -238,6 +484,37 @@ Section SimRelCertStepLemma.
     unfolder. ins. desf.
     { eapply basic_step_e2a_lab_e with (S:=S); eauto; apply SRCC. }
     eapply basic_step_e2a_lab_e' with (S:=S); eauto; apply SRCC.
+  Qed.
+
+  Lemma simrel_cert_forwarding_jf_in_cert_rf lbl lbl' k k' e e' S 
+        (st st' st'': (thread_st (ktid S k)))
+        (SRCC : simrel_cert prog S G sc TC TC' X k st st'')
+        (FRWD : forwarding S lbl lbl' k k' e e' st st')         
+        (CST_REACHABLE : (lbl_step (ktid S k))＊ st' st'') :
+    e2a S □ (Sjf S ⨾ ⦗kE S k'⦘) ⊆ cert_rf G sc TC' (ktid S k').
+  Proof.
+    assert (ES.Wf S) as WF.
+    { apply SRCC. }
+    assert (simrel_cont (stable_prog_to_prog prog) S G TC X) 
+      as SRCONT.
+    { apply SRCC. } 
+    assert (ES.cont_adjacent S k k' e e') as ADJ.
+    { apply FRWD. }
+    arewrite (ktid S k' = ktid S k).
+    { symmetry. apply ADJ. }
+    erewrite ES.cont_adjacent_sb_dom; eauto.
+    rewrite !id_union, !seq_union_r, !collect_rel_union.
+    unionL; auto.
+    { apply SRCC. }
+    { apply FRWD. }
+    unfold eq_opt.
+    destruct e' as [e'|].
+    2 : basic_solver.
+    assert (ES.rmw S e e') as RMW.
+    { eapply ES.cont_adjacent_rmw; eauto. }
+    apply ES.rmwD in RMW; auto.
+    rewrite ES.jfD; auto.
+    generalize RMW. type_solver. 
   Qed.
 
   Lemma simrel_cert_step_jf_in_cert_rf k k' e e' S S'
@@ -286,6 +563,49 @@ Section SimRelCertStepLemma.
     { basic_solver. }
     desf. simpls. desf. unfolder. ins. desf. omega.
   Qed.
+
+  Lemma simrel_cert_forwarding_ex_cont_iss lbl lbl' k k' e e' S 
+        (st st' st'': (thread_st (ktid S k)))
+        (SRCC : simrel_cert prog S G sc TC TC' X k st st'')
+        (FRWD : forwarding S lbl lbl' k k' e e' st st')         
+        (CST_REACHABLE : (lbl_step (ktid S k))＊ st' st'') :
+    X ∩₁ e2a S ⋄₁ (acts_set st'.(ProgToExecution.G) ∩₁ I) ⊆₁ dom_rel (Sew S ⨾ ⦗ kE S k' ⦘).
+  Proof. 
+    assert (ES.Wf S) as WFS.
+    { apply SRCC. }
+    assert (Execution.t S X) as EXEC.
+    { apply SRCC. }
+    assert (simrel_cont (stable_prog_to_prog prog) S G TC X) 
+      as SRCONT.
+    { apply SRCC. }
+    assert (ES.cont_adjacent S k k' e e') as ADJ.
+    { apply FRWD. }
+    erewrite ES.cont_adjacent_sb_dom; eauto.
+    edestruct ilbl_step_acts_set as [a [a' HH]].
+    { eapply wf_cont_state; eauto. }
+    { eapply FRWD. }
+    destruct HH as [EQa [EQa' ACTS]].
+    red in EQa, EQa', ACTS. 
+    rewrite ACTS.
+    rewrite !set_inter_union_l, !set_map_union.
+    rewrite !set_inter_union_r, !id_union, 
+    !seq_union_r, !dom_union.
+    apply set_union_Proper;
+      [apply set_union_Proper|].
+    { apply SRCC. }
+    { intros x [Xx [EQx Ix]].
+      assert (x = e) as EQe.
+      { edestruct e2a_eq_in_cf
+          with (x := x) (y := e) as [EQ | CF]; eauto.
+        { eapply Execution.ex_inE; eauto. }
+        { eapply ES.cont_adjacent_ninit_e; eauto. }
+        { rewrite <- EQx.
+          erewrite forwarding_e2a_e; eauto. }
+        exfalso. 
+        admit. }
+      admit. }
+    admit. 
+  Admitted.
 
   Lemma simrel_cert_step_rmw_cov_in_kE k k' e e' S S'
         (st st' st'': (thread_st (ktid S k)))
@@ -388,267 +708,6 @@ Section SimRelCertStepLemma.
     unfold eq_opt. basic_solver. 
   Qed.
 
-  (* TODO: move to EventStructure.v *)
-  Definition cont_adjacent S k k' e e' := 
-    ⟪ kREP' : k' = CEvent (opt_ext e e') ⟫ /\ 
-    ⟪ kEQTID : ES.cont_thread S k = ES.cont_thread S k' ⟫ /\
-    ⟪ nINITe : SEninit S e ⟫ /\
-    ⟪ RMWe : eq e × eq_opt e' ⊆ Srmw S ⟫ /\
-    ⟪ kSBRMW : ES.cont_sb_dom S k ≡₁ dom_rel (Ssb S ⨾ ⦗eq e⦘) ⟫.
-
-  Lemma cont_adjacent_rmw S (WF : ES.Wf S) k k' e e' 
-        (ADJ : cont_adjacent S k k' e (Some e')) :
-     Srmw S e e'.
-  Proof. 
-    unfold cont_adjacent in ADJ; desc. 
-    apply RMWe. basic_solver.
-  Qed.
-
-  Lemma cont_adjacent_ninit_e S (WF : ES.Wf S) k k' e e' 
-        (ADJ : cont_adjacent S k k' e e') :
-     SEninit S e.
-  Proof. by unfold cont_adjacent in ADJ; desc. Qed.
-
-  Lemma cont_adjacent_ninit_e' S (WF : ES.Wf S) k k' e e' 
-        (ADJ : cont_adjacent S k k' e (Some e')) :
-     SEninit S e'.
-  Proof. 
-    pose proof (cont_adjacent_rmw WF ADJ) as RMW.
-    apply ES.rmwEninit in RMW; auto.
-    generalize RMW. basic_solver. 
-  Qed.
-
-  Lemma cont_adjacent_tid_e S (WF : ES.Wf S) k k' e e' 
-        (ADJ : cont_adjacent S k k' e e') :
-     Stid S e = ES.cont_thread S k.
-  Proof. 
-    unfold cont_adjacent in ADJ; desc.
-    rewrite kEQTID. subst k'.
-    unfold ES.cont_thread, opt_ext in *.
-    destruct e' as [e'|]; auto.
-    apply ES.rmwt; auto.
-    apply RMWe. basic_solver. 
-  Qed.
-
-  Lemma cont_adjacent_tid_e' S (WF : ES.Wf S) k k' e e' 
-        (ADJ : cont_adjacent S k k' e (Some e')) :
-    Stid S e' = ES.cont_thread S k.
-  Proof. 
-    unfold cont_adjacent in ADJ; desc.
-    rewrite kEQTID. subst k'.
-    unfold ES.cont_thread, opt_ext in *; auto.
-  Qed.
-
-  (* TODO: move to AuxRel *)
-  Lemma immediate_transp {A : Type} (r : relation A) : 
-    (immediate r)⁻¹ ≡ immediate (r⁻¹).
-  Proof. basic_solver. Qed.
-
-  Lemma immediate_tsb_functional S (WF : ES.Wf S) x y z 
-        (nINITy  : SEninit S y)
-        (IMMtSB  : immediate (ES.sb S)⁻¹ x y)
-        (IMMtSB' : immediate (ES.sb S)⁻¹ x z) : 
-    y = z.
-  Proof. 
-    destruct IMMtSB  as [SB  nSB ].
-    destruct IMMtSB' as [SB' nSB'].
-    unfold transp in *.
-    assert (SEninit S z) as nINITz.
-    { red. split.
-      { apply ES.sbE in SB'; auto.
-        generalize SB'. basic_solver. }
-      intros INITz.
-      eapply (nSB' y); auto.
-      apply ES.sb_init; auto.
-      basic_solver. }
-    edestruct ES.sb_prcl 
-      as [EQ | HH]; eauto.
-    { split; eauto.
-      eapply ES.sb_tid; auto.
-      basic_solver. }
-    { split; eauto.
-      eapply ES.sb_tid; auto.
-      basic_solver. }
-    destruct HH as [[HH _] | [HH _]].
-    { exfalso. eapply nSB; eauto. }
-    exfalso. eapply (nSB' y); auto.
-  Qed.
-
-  Lemma cont_adjacent_sb_dom S (WF : ES.Wf S) k k' e e'
-        (ADJ : cont_adjacent S k k' e e') :
-    ES.cont_sb_dom S k' ≡₁ ES.cont_sb_dom S k ∪₁ eq e ∪₁ eq_opt e'.
-  Proof. 
-    red in ADJ. desc. subst k'.
-    unfold ES.cont_sb_dom at 1.
-    unfold opt_ext, eq_opt in *.
-    destruct e' as [e'|].
-
-    { assert (Srmw S e e') as RMW.
-      { generalize RMWe. basic_solver. }
-      rewrite crE. relsf.
-      rewrite set_unionC.
-      apply set_union_Propere; auto.
-      arewrite (dom_rel (Ssb S ⨾ ⦗eq e'⦘) ≡₁ 
-                        dom_rel ((Ssb S)^? ⨾ ⦗eq e⦘)).
-      { split.
-        { rewrite ES.sb_imm_split_r at 1; auto. 
-          rewrite !seqA, !seq_eqv_r.
-          intros x [y [z [SB [IMMSB EQy]]]].
-          subst y. exists z. 
-          splits; auto.
-          eapply immediate_tsb_functional; eauto.
-          { apply immediate_transp with (r := Ssb S). red.
-            eapply ES.rmwi; eauto. }
-          apply immediate_transp with (r := Ssb S). by red. }
-        rewrite crE. relsf. 
-        rewrite !seq_eqv_r. splits.
-        { unfolder. ins. desf.
-          eexists; splits; eauto.
-          apply ES.rmw_in_sb; auto. }
-        unfolder. ins. desf.
-        exists e'; splits; eauto.
-        eapply ES.sb_trans; eauto.
-        apply ES.rmw_in_sb; auto. }
-      rewrite crE. relsf.
-      rewrite set_unionC.
-      apply set_union_Propere; auto.
-      by rewrite kSBRMW. }
-
-    rewrite crE. relsf.
-    rewrite set_unionC.
-    apply set_union_Propere; auto.
-    by rewrite kSBRMW.
-  Qed.
-
-  Lemma cont_adjacent_sb_dom_mon S (WF : ES.Wf S) k k' e e'
-        (ADJ : cont_adjacent S k k' e e') :
-    ES.cont_sb_dom S k ⊆₁ ES.cont_sb_dom S k'.
-  Proof. 
-    erewrite cont_adjacent_sb_dom 
-      with (k' := k'); eauto.
-    basic_solver.
-  Qed.
-
-  Definition forwarding S lbl lbl' k k' e e'
-             (st st' : thread_st (ktid S k)) :=
-    ⟪ LBL  : lbl  = Slab S e ⟫ /\
-    ⟪ LBL' : lbl' = option_map (Slab S) e' ⟫ /\
-    ⟪ Kk   : K S (k , existT _ _ st ) ⟫ /\
-    ⟪ Kk'  : K S (k', existT _ _ st') ⟫ /\
-    ⟪ ADJ  : cont_adjacent S k k' e e'⟫ /\
-    ⟪ STEP : ilbl_step (ktid S k) (opt_to_list lbl' ++ [lbl]) st st' ⟫ /\  
-    ⟪ CertRF : e2a S □ Sjf S ⨾ ⦗eq e⦘ ⊆ cert_rf G sc TC' (ktid S k) ⟫.  
-
-  Lemma forwarding_seqn_e S lbl lbl' k k' e e'
-             (st st' st'': thread_st (ktid S k))
-             (SRCC : simrel_cert prog S G sc TC TC' X k st st'')
-             (FRWD : forwarding S lbl lbl' k k' e e' st st') :
-    ES.seqn S e = eindex st.
-  Proof. 
-    assert (ES.Wf S) as WF.
-    { apply SRCC. }
-    assert (simrel_cont (stable_prog_to_prog prog) S G TC X) 
-      as SRCONT.
-    { apply SRCC. }
-    unfold forwarding in FRWD. desc.
-    set (AA := ADJ).
-    unfold cont_adjacent in AA. desc.
-    unfold ES.cont_sb_dom in kSBRMW.
-    destruct k eqn:Heq.
-    { erewrite continit; eauto.
-      unfold ES.seqn.
-      arewrite (dom_rel (Ssb S ∩ ES.same_tid S ⨾ ⦗eq e⦘) ≡₁ ∅).
-      2 : by erewrite countNatP_empty.
-      split; [|done].
-      rewrite seq_eqv_r.
-      intros x [y [[SB STID] EQy]].
-      red. subst y.
-      eapply ES.init_tid_K; eauto.
-      exists (existT _ _ st), k.
-      splits; [by subst k|]. 
-      subst k. erewrite <- cont_adjacent_tid_e; eauto.
-      rewrite <- STID.
-      assert (SEinit S x) as INITx.
-      { apply kSBRMW. basic_solver 10. }
-      red in INITx. unfolder in INITx. desf. }
-    erewrite contseqn; eauto.
-    erewrite ES.seqn_immsb; eauto.
-    { red. 
-      erewrite cont_adjacent_tid_e 
-        with (k := k) (e := e); eauto.
-      2 : eby subst k.
-      unfold ES.cont_thread. desf. }
-    red. splits.
-    { assert (dom_rel (Ssb S ⨾ ⦗eq e⦘) eid) as HH.
-      { apply kSBRMW. basic_solver 10. }
-      unfolder in HH. desf. } 
-    intros x SB SB'.
-    assert (dom_rel ((Ssb S)^? ⨾ ⦗eq eid⦘) x) as HH.
-    { apply kSBRMW. basic_solver 10. }
-    unfolder in HH. desf.
-    { eapply ES.sb_irr; eauto. }
-    eapply ES.sb_irr; eauto.
-    eapply ES.sb_trans; eauto.
-  Qed.
-
-  Lemma forwarding_seqn_e' S lbl lbl' k k' e e'
-        (st st' st'': thread_st (ktid S k))
-        (SRCC : simrel_cert prog S G sc TC TC' X k st st'')
-        (FRWD : forwarding S lbl lbl' k k' e (Some e') st st') :
-    ES.seqn S e' = 1 + eindex st.
-  Proof. 
-    assert (ES.Wf S) as WF.
-    { apply SRCC. }
-    assert (simrel_cont (stable_prog_to_prog prog) S G TC X) 
-      as SRCONT.
-    { apply SRCC. }
-    set (AA := FRWD).
-    unfold forwarding in AA. desc.
-    set (AA := ADJ).
-    unfold cont_adjacent in AA. desc.
-    assert (immediate (ES.sb S) e e') as IMMSB.
-    { apply ES.rmwi; auto.
-      apply RMWe. basic_solver. }
-    erewrite ES.seqn_immsb 
-      with (x := e); eauto; try red; splits.
-    { erewrite forwarding_seqn_e; eauto. }
-    erewrite cont_adjacent_tid_e; eauto. 
-    erewrite cont_adjacent_tid_e'
-      with (k := k); eauto. 
-  Qed.
-
-  Lemma forwarding_e2a_e S lbl lbl' k k' e e'
-             (st st' st'': thread_st (ktid S k))
-             (SRCC : simrel_cert prog S G sc TC TC' X k st st'')
-             (FRWD : forwarding S lbl lbl' k k' e e' st st') :
-    e2a S e = ThreadEvent (ES.cont_thread S k) (eindex st).
-  Proof. 
-    assert (ES.Wf S) as WF.
-    { apply SRCC. }
-    assert (cont_adjacent S k k' e e') as ADJ.
-    { apply FRWD. }
-    rewrite e2a_ninit; auto.
-    2 : eapply cont_adjacent_ninit_e; eauto.
-    erewrite cont_adjacent_tid_e; eauto.
-    erewrite forwarding_seqn_e; eauto.
-  Qed.
-
-  Lemma forwarding_e2a_e' S lbl lbl' k k' e e'
-        (st st' st'': thread_st (ktid S k))
-        (SRCC : simrel_cert prog S G sc TC TC' X k st st'')
-        (FRWD : forwarding S lbl lbl' k k' e (Some e') st st') :
-    e2a S e' = ThreadEvent (ES.cont_thread S k) (1 + eindex st).
-  Proof. 
-    assert (ES.Wf S) as WF.
-    { apply SRCC. }
-    assert (cont_adjacent S k k' e (Some e')) as ADJ.
-    { apply FRWD. }
-    rewrite e2a_ninit; auto.
-    2 : eapply cont_adjacent_ninit_e'; eauto.
-    erewrite cont_adjacent_tid_e'; eauto.
-    erewrite forwarding_seqn_e'; eauto.
-  Qed.
-
   Lemma simrel_cert_forwarding lbl lbl' k k' e e' S
         (st st' st'': thread_st (ktid S k))
         (SRCC : simrel_cert prog S G sc TC TC' X k st st'')
@@ -679,11 +738,10 @@ Section SimRelCertStepLemma.
     assert (Gtid (e2a S e) = ES.cont_thread S k) as GTIDe.
     { erewrite e2a_ninit; [|apply ADJ].
       unfold Events.tid.
-      erewrite cont_adjacent_tid_e; eauto. }
+      erewrite ES.cont_adjacent_tid_e; eauto. }
     
     constructor; auto. 
-    all: try rewrite <- kEQTID.
-    all: try apply SRCC.
+    all: try (by try rewrite <- kEQTID; apply SRCC).
     (* cstate : simrel_cstate S k' st' st'' *)      
     { constructor. 
       { eapply cstate_stable, SRCC. }
@@ -691,118 +749,15 @@ Section SimRelCertStepLemma.
           by rewrite <- kEQTID. }
         by rewrite <- kEQTID. }
     (* ex_ktid_cov : X ∩₁ STid ktid' ∩₁ e2a ⋄₁ C ⊆₁ kE' *)
-    { etransitivity; [apply SRCC|].
-      eapply cont_adjacent_sb_dom_mon; eauto. }
+    { eapply simrel_cert_forwarding_ex_ktid_cov; eauto. }
     (* cov_in_ex : e2a ⋄₁ C ∩₁ kE' ⊆₁ X *)
-    { rewrite cont_adjacent_sb_dom 
-        with (k' := k'); eauto.
-      rewrite set_unionA.
-      rewrite set_inter_union_r.
-      unionL.
-      { rewrite set_interC. 
-        rewrite set_interC. 
-        apply SRCC. }
-      rewrite set_inter_union_r. 
-      unfolder. unionL.
-      { intros x [Cx EQx]. subst x. exfalso. 
-        eapply e2a_ge_ncov; eauto.
-        { apply FRWD. }
-        { erewrite cont_adjacent_tid_e; eauto. }
-        erewrite forwarding_seqn_e; eauto. }
-      intros x [Cx EQx].
-      destruct e' as [e'|]; [|done].
-      subst x. exfalso. 
-      eapply e2a_ge_ncov; eauto.
-      { eapply cont_adjacent_ninit_e'; eauto. }
-      { erewrite cont_adjacent_tid_e'; eauto. }
-      erewrite forwarding_seqn_e'; eauto. }
+    { eapply simrel_cert_forwarding_cov_in_ex; eauto. }
     (* kE_lab : eq_dom (kE' \₁ SEinit) Slab (certG.(lab) ∘ e2a) *)
-    { rewrite cont_adjacent_sb_dom 
-        with (k' := k'); eauto.
-      rewrite set_unionA.
-      rewrite !set_minus_union_l.
-      rewrite !eq_dom_union. splits.
-      { apply SRCC. }
-      { intros x [EQx _]. subst x.
-        unfold compose.
-        erewrite steps_preserve_lab; eauto.
-        { rewrite <- LBL.
-          erewrite forwarding_e2a_e; eauto.
-          eapply ilbl_step_eindex_lbl; eauto. }
-        { by rewrite GTIDe. }
-        { apply lbl_steps_in_steps. 
-            by rewrite GTIDe. }
-        erewrite forwarding_e2a_e; eauto.
-        eapply acts_clos; eauto.
-        eapply ilbl_step_eindex_lt.
-        apply STEP. }
-      intros x [EQx _]. 
-      unfold eq_opt in EQx. 
-      destruct e' as [e'|]; [|done]. 
-      assert (Gtid (e2a S e') = ES.cont_thread S k) as GTIDe'.
-      { erewrite e2a_ninit.
-        2 : eapply cont_adjacent_ninit_e'; eauto.
-        unfold Events.tid.
-        erewrite cont_adjacent_tid_e'; eauto. }
-      subst x. unfold compose.
-      erewrite steps_preserve_lab; eauto.
-      { unfold option_map in LBL'.
-        destruct lbl' as [lbl'|]; 
-          inversion LBL' as [HLBL'].
-        rewrite <- HLBL'.
-        erewrite forwarding_e2a_e'; eauto.
-        eapply ilbl_step_eindex_lbl'; eauto. }
-      { by rewrite GTIDe'. }
-      { apply lbl_steps_in_steps. 
-          by rewrite GTIDe'. }
-      erewrite forwarding_e2a_e'; eauto.
-      eapply acts_clos; eauto.
-      erewrite ilbl_step_eindex_shift
-        with (st' := st'); eauto.
-      unfold option_map in LBL'.
-      destruct lbl' as [lbl'|].
-      2 : inversion LBL'.
-      unfold opt_to_list, app, length.
-      omega. }
+    { eapply simrel_cert_forwarding_kE_lab; eauto. }
     (* jf_in_cert_rf : e2a □ (Sjf ⨾ ⦗kE'⦘) ⊆ cert_rf G sc TC' ktid' *)
-    { erewrite cont_adjacent_sb_dom; eauto.
-      rewrite !id_union, !seq_union_r, !collect_rel_union.
-      unionL; auto.
-      { apply SRCC. }
-      unfold eq_opt.
-      destruct e' as [e'|].
-      2 : basic_solver.
-      assert (ES.rmw S e e') as RMW.
-      { eapply cont_adjacent_rmw; eauto. }
-      apply ES.rmwD in RMW; auto.
-      rewrite ES.jfD; auto.
-      generalize RMW. type_solver. }
+    { eapply simrel_cert_forwarding_jf_in_cert_rf; eauto. }
     (* ex_cont_iss : X ∩₁ e2a ⋄₁ (contE' ∩₁ I) ⊆₁ dom_rel (Sew ⨾ ⦗ kE' ⦘) *)
-    { erewrite cont_adjacent_sb_dom; eauto.
-      edestruct ilbl_step_acts_set as [a [a' HH]].
-      { apply WFst. }
-      { edone. }
-      destruct HH as [EQa [EQa' ACTS]].
-      red in EQa, EQa', ACTS. 
-      rewrite ACTS.
-      rewrite !set_inter_union_l, !set_map_union.
-      rewrite !set_inter_union_r, !id_union, 
-              !seq_union_r, !dom_union.
-      apply set_union_Proper;
-        [apply set_union_Proper|].
-      { apply SRCC. }
-      { intros x [Xx [EQx Ix]].
-        assert (x = e) as EQe.
-        { edestruct e2a_eq_in_cf
-            with (x := x) (y := e) as [EQ | CF]; eauto.
-          { eapply Execution.ex_inE; eauto. }
-          { eapply cont_adjacent_ninit_e; eauto. }
-          { rewrite <- EQx.
-            erewrite forwarding_e2a_e; eauto. }
-          exfalso. 
-          admit. }
-        admit. }
-      admit. }
+    { eapply simrel_cert_forwarding_ex_cont_iss; eauto. }
     (* rmw_cov_in_kE : Grmw ⨾ ⦗C' ∩₁ e2a □₁ kE'⦘ ⊆ e2a □ Srmw ⨾ ⦗kE'⦘ *)
     { erewrite cont_adjacent_sb_dom; eauto.
       rewrite !set_collect_union.
