Coq/src/AuxRel.v
@@ -866,6 +866,10 @@ Lemma immediate_inter :
   (immediate r) ∩ r' ⊆ immediate (r ∩ r').
 Proof. basic_solver. Qed.
 
+Lemma immediate_transp :
+  (immediate r)⁻¹ ≡ immediate (r⁻¹).
+Proof. basic_solver. Qed.
+
 Lemma trans_prcl_immediate_seqr_split x y
       (TRANS : transitive r) (PRCL : downward_total r) (IMM : (immediate r) x y) :
   r ⨾ ⦗ eq y ⦘ ≡ (eq x ∪₁ dom_rel (r ⨾ ⦗ eq x ⦘)) × eq y.
